theories/Temporal.v
@@ -1,4 +1,4 @@
-From Coq Require Import Lists.List.
+From Coq Require Import Lists.List Lia Classes.Morphisms Bool.Bool.
 From Mecha Require Import RFlows REnvironment Term Functional Resource Cell Typing VContext Typ
                Resources Evaluation RContext RFlow.
 
@@ -43,16 +43,139 @@ Inductive wf_env_TT : ℜ -> 𝐅 -> Prop :=
       Wfₜₜ(Re,Fl) ->
       Addᵣᵪ (newᵣᵪ(Re)) (τ,τ') Re Re' ->
       Addᵣₔ (newᵣₔ(Fl)) r Fl Fl' ->
-      RFlow.inp_wt Re τ' r ->
-      RFlow.out_wt Re τ r ->
+      RFlow.well_typed_rflow (∅ᵥᵪ) Re r τ' τ ->
       Wfₜₜ(Re',Fl')
 
-  | wfTT_update : forall (Re : ℜ) V (Fl : 𝐅),
-      Wfₜₜ(Re,Fl) ->
-      Wfᵣₜ(Re,V) ->
-      Wfₜₜ(Re,(RFlows.puts V Fl))
-
 where "'Wfₜₜ(' Re , Fl )" := (wf_env_TT Re Fl).
+
+(** *** wf_env_TT *)
+
+Lemma wf_env_TT_is_empty_spec : forall (Re : ℜ) Fl,
+  Wfₜₜ(Re,Fl) -> RC.Raw.is_empty Re = RFlows.Raw.is_empty Fl.
+Proof.
+  intros Re V Hinst; induction Hinst.
+  - rewrite RC.OP.P.is_empty_1; auto; 
+    now rewrite RFlows.OP.P.is_empty_1.
+  - apply RC.notEmpty_Add_spec in H.
+    apply RFlows.notEmpty_Add_spec in H0.
+    destruct (RC.Raw.is_empty Re') eqn:HEmp.
+    -- apply RC.OP.P.is_empty_2 in HEmp; contradiction.
+    -- destruct (RFlows.Raw.is_empty Fl') eqn:HEmp'; auto.
+        apply RFlows.OP.P.is_empty_2 in HEmp'; contradiction.
+Qed.
+
+Lemma wf_env_TT_Empty_spec : forall (Re : ℜ) Fl,
+  Wfₜₜ(Re,Fl) -> isEmptyᵣᵪ(Re) <-> isEmptyᵣₔ(Fl).
+Proof.
+  intros Re V Hinst; induction Hinst.
+  - split; intros; assumption.
+  - split; intros.
+    -- now apply RC.notEmpty_Add_spec in H.
+    -- now apply RFlows.notEmpty_Add_spec in H0.
+Qed.
+
+Lemma wf_env_TT_max : forall (Re : ℜ) Fl,
+  Wfₜₜ(Re,Fl) -> maxᵣᵪ(Re) = maxᵣₔ(Fl).
+Proof.
+  intros Re V inst; induction inst.
+  - rewrite RC.Ext.max_key_Empty_spec; auto.
+    now rewrite RFlows.Ext.max_key_Empty_spec.
+  - apply RC.Ext.max_key_Add_spec in H as [[H H'] | [H H']]; auto.
+    -- rewrite H. 
+        apply RFlows.Ext.max_key_Add_spec in H0 as [[H0 H0'] | [H0 H0']].
+        + rewrite H0; apply wf_env_TT_is_empty_spec in inst as HEmp.
+          unfold RC.Ext.new_key,RFlows.Ext.new_key; rewrite HEmp.
+          destruct (RFlows.Raw.is_empty Fl); auto.
+        + assert (newᵣₔ(Fl) >= maxᵣₔ(Fl)). { apply RFlows.Ext.new_key_geq_max_key. }
+          lia.
+        + apply RFlows.new_key_notin_spec; auto.
+    -- unfold RC.Ext.new_key in H'. 
+        destruct (RC.Raw.is_empty Re) eqn:HEmp; try lia.
+        rewrite RC.Ext.max_key_Empty_spec in H'; try lia.
+        now apply RC.OP.P.is_empty_2.
+    -- apply RC.Ext.new_key_notin_spec; lia.
+Qed.
+
+Lemma wf_env_TT_new : forall (Re : ℜ) Fl,
+  Wfₜₜ(Re,Fl) -> newᵣᵪ(Re) = newᵣₔ(Fl).
+Proof.
+  intros Re Fl Hwf; unfold RC.Ext.new_key,RFlows.Ext.new_key.
+  apply wf_env_TT_is_empty_spec in Hwf as HisEmp.
+  destruct (RC.Raw.is_empty Re) eqn:HEmp.
+  - now rewrite <- HisEmp.
+  - rewrite <- HisEmp; f_equal; now apply wf_env_TT_max.
+Qed.
+
+Lemma wf_env_TT_domains_match: forall (Re : ℜ) Fl (k : resource) (πτ : πΤ),
+  Wfₜₜ(Re,Fl) -> Re ⌈k ⩦ πτ⌉ᵣᵪ -> exists v, Fl ⌈k ⩦ v⌉ᵣₔ.
+Proof.
+  intros Re Fl k πτ wf; revert k πτ; induction wf; intros k' πτ' Hfin.
+  - apply RC.notEmpty_find_spec in Hfin; auto; contradiction.
+  - rewrite H0 in *; destruct (Resource.eq_dec (newᵣᵪ(Re)) k'); subst.
+    -- exists r. 
+       apply wf_env_TT_new in wf as Hnew; rewrite Hnew.
+       now apply RFlows.OP.P.add_eq_o.
+    -- rewrite H in Hfin. rewrite RC.OP.P.add_neq_o in Hfin; try assumption.
+        apply IHwf in Hfin as [v' Hfin]; exists v'. 
+        rewrite RFlows.OP.P.add_neq_o; auto.
+        apply wf_env_TT_new in wf; now rewrite <- wf.
+Qed.
+
+#[export] 
+Instance wfTT_eq : Proper (RC.eq ==> RFlows.eq ==> iff) (wf_env_TT).
+Proof.
+  repeat red; split; intros.
+  - revert y y0 H0 H; induction H1; subst; intros y y0 Heq Heq'.
+    -- apply wfTT_empty; try (now rewrite <- Heq); now rewrite <- Heq'.
+    -- eapply wfTT_add; eauto; try (now rewrite <- Heq); now rewrite <- Heq'.
+  - revert x x0 H0 H; induction H1; subst; intros x x0 Heq Heq'.
+    -- apply wfTT_empty; try (now rewrite Heq'); now rewrite Heq.
+    -- eapply wfTT_add; eauto; try (now rewrite Heq); now rewrite Heq'.
+Qed.
+
+Lemma wf_env_TT_in : forall (Re : ℜ) Fl (r : resource),
+  Wfₜₜ(Re,Fl) -> r ∈ᵣᵪ Re <-> r ∈ᵣₔ Fl.
+Proof.
+  split.
+  - intros; destruct H0; apply RC.OP.P.find_1 in H0. 
+    eapply wf_env_TT_domains_match in H0; eauto;
+    destruct H0. exists x0; now apply RFlows.OP.P.find_2.
+  - revert r; induction H.
+    -- intros. unfold RE.OP.P.Empty in *; exfalso.
+       destruct H1. now apply (H0 r x).
+    -- intros. unfold RFlows.OP.P.Add in *. rewrite H1 in *.
+       unfold RC.OP.P.Add in *. rewrite H0.
+       apply RFlows.OP.P.add_in_iff in H3; destruct H3; subst.
+       + apply wf_env_TT_new in H; rewrite H.
+         rewrite RC.OP.P.add_in_iff; now left.
+       + rewrite RC.OP.P.add_in_iff; right; now apply IHwf_env_TT.
+Qed.
+
+
+Lemma wf_env_TT_well_typed : forall (Re : ℜ) Fl (r : resource) v (τ τ' : Τ),
+  Wfₜₜ(Re,Fl) -> Re ⌈r ⩦ (τ,τ')⌉ᵣᵪ -> Fl ⌈r ⩦ v⌉ᵣₔ -> 
+  RFlow.well_typed_rflow (∅ᵥᵪ) Re v τ' τ.
+Proof.
+  intros Re V r v τ τ' wf; revert r v τ τ'; induction wf;
+  intros r' v' τ1 τ1' HfRe HfFl.
+  - apply RC.notEmpty_find_spec in HfRe; auto; contradiction.
+  - rewrite H in HfRe; rewrite H0 in HfFl.
+    apply wf_env_TT_new in wf as Hnew. 
+    destruct (Resource.eq_dec (newᵣᵪ(Re)) r'); subst.
+    -- rewrite Hnew in HfFl. rewrite RC.OP.P.add_eq_o in HfRe; auto; 
+        inversion HfRe; clear HfRe; subst.
+        rewrite RFlows.OP.P.add_eq_o in HfFl; auto; inversion HfFl; 
+        subst; clear HfFl. apply RFlow.rflow_weakening_ℜ with (Re := Re); auto.
+        unfold RC.OP.P.Add in H. rewrite H. apply RC.Ext.Submap_add_spec_1.
+        + apply RC.Ext.new_key_notin_spec; lia.
+        + reflexivity.
+    -- rewrite <- Hnew in HfFl. rewrite RC.OP.P.add_neq_o in HfRe; auto.
+        rewrite RFlows.OP.P.add_neq_o in HfFl; auto. eapply IHwf in HfFl; eauto.
+        apply RFlow.rflow_weakening_ℜ with (Re := Re); auto.
+        unfold RC.OP.P.Add in H. rewrite H. apply RC.Ext.Submap_add_spec_1.
+        + apply RC.Ext.new_key_notin_spec; lia.
+        + reflexivity.
+Qed.
 
 Lemma wf_env_TT_to_fT Re Fl : 
   Wfₜₜ(Re,Fl) -> Wfᵣₜ(Re,RFlows.nexts Fl).
@@ -67,7 +190,71 @@ Proof.
        + apply RFlows.new_key_notin_spec; auto.
        + assumption.
     -- destruct r; simpl in *; apply H2.
-  - 
+Qed.
+
+Lemma wf_env_fT_update (Re : ℜ) V (Fl Fl' : 𝐅): 
+  Wfₜₜ(Re,Fl) ->  Wfᵣₜ(Re,V) ->
+  (Fl' = (RFlows.puts V Fl))%rf -> Wfₜₜ(Re,Fl').
+Proof.
+  intros wftt; revert Fl' V; induction wftt; intros Fl1 V Hwfrt Heq.
+  - rewrite RFlows.puts_Empty_eq with (V := V) in H0.
+    apply wfTT_empty; auto; rewrite Heq; auto.
+  -
+    rename H into HAddRe; rename H0 into HAddFl; move Fl1 before Fl;
+    move V before Re'; move IHwftt before r; move Hwfrt before wftt;
+    rename H1 into Hwtr; move Hwtr before IHwftt.
+
+    assert(HInRe': (newᵣᵪ(Re)) ∈ᵣᵪ Re').
+    { exists (τ,τ'). apply RC.OP.P.find_2. rewrite HAddRe. now rewrite RC.OP.P.add_eq_o. }
+
+    move HInRe' before HAddFl.
+    
+    assert (Hnm: newᵣᵪ(Re) = maxᵣᵦ(V)).
+    { 
+     apply wf_env_fT_max in Hwfrt as Hmax. rewrite <- Hmax.
+     apply RC.max_key_Add_spec in HAddRe.
+     - destruct HAddRe as [[Heq' Hle] | [Heq' Hle]]; try lia.
+       assert (newᵣᵪ(Re) >= maxᵣᵪ(Re)) by apply RC.Ext.new_key_geq_max_key.
+       lia.
+     - apply RC.Ext.new_key_notin_spec; auto. 
+    }
+
+    assert (Hnew: maxᵣᵦ(V) = newᵣᵦ(RE.Raw.remove (maxᵣᵦ(V)) V)).
+    { admit. }
+       
+    remember (RE.Raw.remove (maxᵣᵦ(V)) V) as V0.
+    rewrite Hnew in HeqV0. move V0 before Re'.
+
+    assert (HAddV: exists v, RE.OP.P.Add (newᵣᵦ(V0)) v V0 V).
+    {
+      rewrite wf_env_fT_in in HInRe'; eauto.
+      rewrite Hnm in HInRe'. rewrite Hnew in HInRe'. 
+      destruct HInRe' as [v HM]. apply RE.OP.P.find_1 in HM. exists v. 
+      unfold RE.OP.P.Add. apply RE.OP.P.add_id in HM. rewrite <- HM. 
+      rewrite <- RE.OP.P.add_remove_1. now rewrite <- HeqV0.
+    }
+
+    destruct HAddV as [v HAddV]. move v before r; move HAddV before HAddRe.
+    eapply wf_env_fT_weakening_bis in Hwfrt as Hwfrt0; eauto.
+    rewrite Hnew in Hwfrt0. rewrite <- HeqV0 in Hwfrt0.
+    assert (RC.Raw.remove (maxᵣᵪ( Re')) Re' = Re)%rc.
+    { admit. }
+    rewrite <- Hnm in Hnew; clear Hnm. rewrite Heq. rewrite H in *. clear H.
+    assert (Hnew': newᵣₔ(Fl) = newᵣᵦ(V0)).
+    { apply wf_env_TT_new in wftt. rewrite <- Hnew; now rewrite <- wftt. }
+    eapply RFlows.puts_Add_spec_2 with (V := V0) (v := v) (V' := V) in HAddFl.
+    -- apply (wfTT_add Re Re' (RFlows.puts V0 Fl) (RFlows.puts V Fl') 
+                     τ τ' (RFlows.puts_func_1 V0 (newᵣₔ(Fl)) r)); auto.
+       + apply IHwftt with (V := V0); auto; reflexivity.
+       + rewrite <- RFlows.puts_new_spec with (V := V0); assumption.
+       + unfold RFlows.puts_func_1; rewrite Hnew'.
+         replace (V0⌊newᵣᵦ(V0)⌋ᵣᵦ) with (@None Cell.t).
+         ++ now apply RFlow.rflow_well_typed_None.
+         ++ symmetry. apply RE.OP.P.not_in_find.
+            apply RE.Ext.new_key_notin_spec; lia.
+    -- apply RFlows.Ext.new_key_notin_spec; lia.
+    -- rewrite Hnew'. apply RE.Ext.new_key_notin_spec; lia.
+    -- now rewrite Hnew'.
 Admitted.
 
 (** *** Initialization *)
@@ -115,14 +302,14 @@ Proof.
     eapply functional_preserves_typing in H0; eauto.
     -- destruct H0 as [_ [_ [HwfV [_ [_ [HwP' [HltP' [_ HltVout]]]]]]]].
        split; auto; split.
-       +  admit.
+       + eapply wf_env_fT_update; eauto. reflexivity.
        + split; auto. apply RFlows.halts_puts; auto.
     -- exists <[unit]>; split; auto.
     -- apply RFlows.halts_nexts in HlRf. eapply RE.halts_eq; eauto.
     -- now rewrite H.
   - apply IHHTT1 in HwP as IH; auto. destruct IH as [HwP' [Hwf' [HlP' HlR']]].
     apply IHHTT2; assumption.
-Admitted. 
+Qed. 
 
 
 Theorem progress_of_temporal (Re : ℜ) (Rf : 𝐅) (P : Λ) (R : resources) :
